Added a theory utp_alpha_pred of alphabetised predicates which is constructed on top of the theory of simple predicates. Also added the lifting operator to both theories. Note that there are no laws yet for alphabetised predicates, not even closure laws.

theories/generic/utp_pred.thy
@@ -35,12 +35,30 @@ definition binding_equiv ::
 
 notation binding_equiv ("_ \<cong> _ on _")
 
+subsection {* Unrestricted Variables *}
+
+definition UNREST ::
+  "('TYPE VAR) set \<Rightarrow> ('VALUE, 'TYPE) PREDICATE \<Rightarrow> bool" where
+"UNREST vs p \<longleftrightarrow> (\<forall> b1 \<in> p . \<forall> b2 \<in> WF_BINDING . b1 \<oplus> b2 on vs \<in> p)"
+
 subsection {* Predicates *}
 
 definition WF_PREDICATE :: "('VALUE, 'TYPE) PREDICATE set" where
 "WF_PREDICATE = {b . b \<subseteq> WF_BINDING}"
 
+definition WF_PREDICATE_OVER ::
+  "('TYPE VAR) set \<Rightarrow>
+   ('VALUE, 'TYPE) PREDICATE set" where
+"WF_PREDICATE_OVER vs = {p . p \<in> WF_PREDICATE \<and> UNREST (VAR - vs) p}"
+
 subsection {* Operators *}
+
+subsubsection {* Shallow Lifting *}
+
+definition LiftP ::
+  "('VALUE, 'TYPE) BINDING_BFUN \<Rightarrow>
+   ('VALUE, 'TYPE) PREDICATE" where
+"LiftP f = {b \<in> WF_BINDING . f b}"
 
 subsubsection {* True and False *}
 
@@ -131,7 +149,7 @@ definition ClosureP ::
 "p \<in> WF_PREDICATE \<longrightarrow>
  ClosureP p = (\<forall>p VAR . p)"
 
-notation ClosureP ("[_]")
+notation ClosureP ("[_]p")
 
 subsubsection {* Refinement *}
 
@@ -141,7 +159,7 @@ definition RefP ::
    ('VALUE, 'TYPE) PREDICATE" where
 "p1 \<in> WF_PREDICATE \<and>
  p2 \<in> WF_PREDICATE \<longrightarrow>
- RefP p1 p2 = [p2 \<Rightarrow>p p1]"
+ RefP p1 p2 = [p2 \<Rightarrow>p p1]p"
 
 notation RefP (infix "\<sqsubseteq>p" 100)
 
@@ -152,14 +170,14 @@ subsubsection {* Tautologies *}
 definition Tautology ::
   "('VALUE, 'TYPE) PREDICATE \<Rightarrow> bool" where
 "p \<in> WF_PREDICATE \<longrightarrow>
- Tautology p \<longleftrightarrow> [p] = true"
+ Tautology p \<longleftrightarrow> [p]p = true"
 
 notation Tautology ("taut _" [50] 50)
 
 definition Contradiction ::
   "('VALUE, 'TYPE) PREDICATE \<Rightarrow> bool" where
 "p \<in> WF_PREDICATE \<longrightarrow>
- Contradiction p \<longleftrightarrow> [p] = false"
+ Contradiction p \<longleftrightarrow> [p]p = false"
 
 notation Contradiction ("contra _" [50] 50)
 
@@ -218,6 +236,14 @@ theorem WF_BINDING_override_on_VAR [simp] :
  b1 \<oplus> b2 on VAR = b2"
 apply (simp add: VAR_def)
 apply (auto)
+done
+
+subsubsection {* Unrest Theorems *}
+
+theorem UNREST_member [intro] :
+"\<lbrakk>p \<in> WF_PREDICATE; b \<in> p; UNREST vs p; b' \<in> WF_BINDING\<rbrakk> \<Longrightarrow>
+ (b \<oplus> b' on vs) \<in> p"
+apply (simp add: UNREST_def)
 done
 
 subsubsection {* Closure Theorems *}
@@ -292,7 +318,7 @@ done
 
 theorem ClosureP_closure [closure, intro!] :
 "\<lbrakk>p \<in> WF_PREDICATE\<rbrakk> \<Longrightarrow>
- [p] \<in> WF_PREDICATE"
+ [p]p \<in> WF_PREDICATE"
 apply (simp add: ClosureP_def)
 apply (auto)
 done
@@ -392,6 +418,14 @@ done
 theorems QuantP_deatomise =
   ExistsP_deatomise
   ForallP_deatomise
+
+subsubsection {* Validation of Soundness *}
+
+theorem TrueP_noteq_FalseP :
+"true \<noteq> false"
+apply (simp add: TrueP_def FalseP_def)
+apply (simp add: WF_BINDING_non_empty)
+done
 
 subsection {* Proof Experiments *}
 
