theories/alpha/utp_alpha_pred.thy
@@ -1,0 +1,257 @@
+(******************************************************************************)
+(* Project: Unifying Theories of Programming                                  *)
+(* File: utp_alpha_pred.thy                                                   *)
+(* Author: Frank Zeyda, University of York (UK)                               *)
+(******************************************************************************)
+
+header {* Alphabetised Predicates *}
+
+theory utp_alpha_pred
+imports "../generic/utp_pred"
+begin
+
+subsection {* Locale @{text "ALPHA_PRED"} *}
+
+locale ALPHA_PRED =
+  PRED "type_rel"
+-- {* Typing Relation for Values *}
+for type_rel :: "'VALUE \<Rightarrow> 'TYPE \<Rightarrow> bool" (infix ":" 50)
+begin
+
+subsubsection {* Alphabets *}
+
+definition WF_ALPHABET :: "('TYPE ALPHABET) set" where
+"WF_ALPHABET = {vs . finite vs}"
+
+subsubsection {* Bindings *}
+
+definition WF_BINDING_BFUN ::
+  "'TYPE ALPHABET \<Rightarrow> ('VALUE, 'TYPE) BINDING_BFUN set" where
+"a \<in> WF_ALPHABET \<longrightarrow>
+ WF_BINDING_BFUN a = {f . \<forall> b1 b2 . b1 \<cong> b2 on a \<longrightarrow> f b1 = f b2}"
+
+subsubsection {* Predicates *}
+
+abbreviation alphabet ::
+  "('VALUE, 'TYPE) ALPHA_PREDICATE \<Rightarrow>
+   ('TYPE ALPHABET)" where
+"alphabet p \<equiv> (fst p)"
+
+notation alphabet ("\<alpha>")
+
+abbreviation predicate ::
+  "('VALUE, 'TYPE) ALPHA_PREDICATE \<Rightarrow>
+   ('VALUE, 'TYPE) PREDICATE" where
+"predicate p \<equiv> (snd p)"
+
+notation predicate ("\<pi>")
+
+definition WF_ALPHA_PREDICATE ::
+  "('VALUE, 'TYPE) ALPHA_PREDICATE set" where
+"WF_ALPHA_PREDICATE =
+ {p . (\<alpha> p) \<in> WF_ALPHABET \<and> (\<pi> p) \<in> WF_PREDICATE_OVER (\<alpha> p)}"
+
+definition WF_ALPHA_PREDICATE_OVER ::
+  "'TYPE ALPHABET \<Rightarrow> ('VALUE, 'TYPE) ALPHA_PREDICATE set" where
+"a \<in> WF_ALPHABET \<longrightarrow>
+ WF_ALPHA_PREDICATE_OVER a = {p . p \<in> WF_ALPHA_PREDICATE \<and> \<alpha> p = a}"
+
+subsection {* Operators *}
+
+subsubsection {* Shallow Lifting *}
+
+definition LiftA ::
+  "'TYPE ALPHABET \<Rightarrow>
+   ('VALUE, 'TYPE) BINDING_BFUN \<Rightarrow>
+   ('VALUE, 'TYPE) ALPHA_PREDICATE" where
+"a \<in> WF_ALPHABET \<and>
+ f \<in> WF_BINDING_BFUN a \<longrightarrow>
+ LiftA a f = (a, LiftP f)"
+
+subsubsection {* Extension and Restriction *}
+
+definition ExtA ::
+  "('VALUE, 'TYPE) ALPHA_PREDICATE \<Rightarrow> 'TYPE ALPHABET \<Rightarrow>
+   ('VALUE, 'TYPE) ALPHA_PREDICATE" where
+"p \<in> WF_ALPHA_PREDICATE \<and>
+ a \<in> WF_ALPHABET \<longrightarrow>
+ ExtA p a = ((\<alpha> p) \<union> a, \<pi> p)"
+
+notation ExtA (infix "\<oplus>\<alpha>" 200)
+
+definition ResA ::
+  "('VALUE, 'TYPE) ALPHA_PREDICATE \<Rightarrow> 'TYPE ALPHABET \<Rightarrow>
+   ('VALUE, 'TYPE) ALPHA_PREDICATE" where
+"p \<in> WF_ALPHA_PREDICATE \<and>
+ a \<in> WF_ALPHABET \<longrightarrow>
+ ResA p a = ((\<alpha> p) - a, \<exists>p a . \<pi> p)"
+
+notation ResA (infix "\<ominus>\<alpha>" 200)
+
+subsubsection {* True and False *}
+
+definition TrueA ::
+  "'TYPE ALPHABET \<Rightarrow> ('VALUE, 'TYPE) ALPHA_PREDICATE" where
+"a \<in> WF_ALPHABET \<longrightarrow>
+ TrueA a = (a, true)"
+
+notation TrueA ("true")
+
+definition FalseA ::
+  "'TYPE ALPHABET \<Rightarrow> ('VALUE, 'TYPE) ALPHA_PREDICATE" where
+"a \<in> WF_ALPHABET \<longrightarrow>
+ FalseA a = (a, false)"
+
+notation FalseA ("false")
+
+subsubsection {* Logical Connectives *}
+
+definition NotA ::
+  "('VALUE, 'TYPE) ALPHA_PREDICATE \<Rightarrow>
+   ('VALUE, 'TYPE) ALPHA_PREDICATE" where
+"p \<in> WF_ALPHA_PREDICATE \<longrightarrow>
+ NotA p = (\<alpha> p, \<not>p (\<pi> p))"
+
+notation NotA ("\<not>\<alpha> _" [190] 190)
+
+definition AndA ::
+  "('VALUE, 'TYPE) ALPHA_PREDICATE \<Rightarrow>
+   ('VALUE, 'TYPE) ALPHA_PREDICATE \<Rightarrow>
+   ('VALUE, 'TYPE) ALPHA_PREDICATE" where
+"p1 \<in> WF_ALPHA_PREDICATE \<and>
+ p2 \<in> WF_ALPHA_PREDICATE \<longrightarrow>
+ AndA p1 p2 = ((\<alpha> p1) \<union> (\<alpha> p2), (\<pi> p1) \<and>p (\<pi> p2))"
+
+notation AndA (infixr "\<and>\<alpha>" 180)
+
+definition OrA ::
+  "('VALUE, 'TYPE) ALPHA_PREDICATE \<Rightarrow>
+   ('VALUE, 'TYPE) ALPHA_PREDICATE \<Rightarrow>
+   ('VALUE, 'TYPE) ALPHA_PREDICATE" where
+"p1 \<in> WF_ALPHA_PREDICATE \<and>
+ p2 \<in> WF_ALPHA_PREDICATE \<longrightarrow>
+ OrA p1 p2 = ((\<alpha> p1) \<union> (\<alpha> p2), (\<pi> p1) \<or>p (\<pi> p2))"
+
+notation OrA (infixr "\<or>\<alpha>" 170)
+
+definition ImpliesA ::
+  "('VALUE, 'TYPE) ALPHA_PREDICATE \<Rightarrow>
+   ('VALUE, 'TYPE) ALPHA_PREDICATE \<Rightarrow>
+   ('VALUE, 'TYPE) ALPHA_PREDICATE" where
+"p1 \<in> WF_ALPHA_PREDICATE \<and>
+ p2 \<in> WF_ALPHA_PREDICATE \<longrightarrow>
+ ImpliesA p1 p2 = ((\<alpha> p1) \<union> (\<alpha> p2), (\<pi> p1) \<Rightarrow>p (\<pi> p2))"
+
+notation ImpliesA (infixr "\<Rightarrow>\<alpha>" 160)
+
+definition IffA ::
+  "('VALUE, 'TYPE) ALPHA_PREDICATE \<Rightarrow>
+   ('VALUE, 'TYPE) ALPHA_PREDICATE \<Rightarrow>
+   ('VALUE, 'TYPE) ALPHA_PREDICATE" where
+"p1 \<in> WF_ALPHA_PREDICATE \<and>
+ p2 \<in> WF_ALPHA_PREDICATE \<longrightarrow>
+ IffA p1 p2 = ((\<alpha> p1) \<union> (\<alpha> p2), (\<pi> p1) \<Leftrightarrow>p (\<pi> p2))"
+
+notation IffA (infixr "\<Leftrightarrow>\<alpha>" 150)
+
+subsubsection {* Quantifiers *}
+
+definition ExistsA ::
+  "'TYPE ALPHABET \<Rightarrow>
+   ('VALUE, 'TYPE) ALPHA_PREDICATE \<Rightarrow>
+   ('VALUE, 'TYPE) ALPHA_PREDICATE" where
+"a \<in> WF_ALPHABET \<and>
+ p \<in> WF_ALPHA_PREDICATE \<longrightarrow>
+ ExistsA a p = ((\<alpha> p), \<exists>p a . \<pi> p)"
+
+notation ExistsA ("(\<exists>\<alpha> _ ./ _)" [0, 10] 10)
+
+definition ForallA ::
+  "'TYPE ALPHABET \<Rightarrow>
+   ('VALUE, 'TYPE) ALPHA_PREDICATE \<Rightarrow>
+   ('VALUE, 'TYPE) ALPHA_PREDICATE" where
+"a \<in> WF_ALPHABET \<and>
+ p \<in> WF_ALPHA_PREDICATE \<longrightarrow>
+ ForallA a p = ((\<alpha> p), \<forall>p a . \<pi> p)"
+
+notation ForallA ("(\<forall>\<alpha> _ ./ _)" [0, 10] 10)
+
+definition ExistsResA ::
+  "('TYPE ALPHABET) \<Rightarrow>
+   ('VALUE, 'TYPE) ALPHA_PREDICATE \<Rightarrow>
+   ('VALUE, 'TYPE) ALPHA_PREDICATE" where
+"a \<in> WF_ALPHABET \<and>
+ p \<in> WF_ALPHA_PREDICATE \<longrightarrow>
+ ExistsResA a p = ((\<alpha> p) - a, \<exists>p a . \<pi> p)"
+
+notation ExistsResA ("(\<exists>-\<alpha> _ ./ _)" [0, 10] 10)
+
+definition ForallResA ::
+  "'TYPE ALPHABET \<Rightarrow>
+   ('VALUE, 'TYPE) ALPHA_PREDICATE \<Rightarrow>
+   ('VALUE, 'TYPE) ALPHA_PREDICATE" where
+"a \<in> WF_ALPHABET \<and>
+ p \<in> WF_ALPHA_PREDICATE \<longrightarrow>
+ ForallResA a p = ((\<alpha> p) - a, \<forall>p a . \<pi> p)"
+
+notation ForallResA ("(\<forall>-\<alpha> _ ./ _)" [0, 10] 10)
+
+subsubsection {* Universal Closure *}
+
+definition ClosureA ::
+  "('VALUE, 'TYPE) ALPHA_PREDICATE \<Rightarrow>
+   ('VALUE, 'TYPE) ALPHA_PREDICATE" where
+"p \<in> WF_ALPHA_PREDICATE \<longrightarrow>
+ ClosureA p = ({}, [\<pi> p]p)"
+
+notation ClosureA ("[_]\<alpha>")
+
+subsubsection {* Refinement *}
+
+definition RefA ::
+  "('VALUE, 'TYPE) ALPHA_PREDICATE \<Rightarrow>
+   ('VALUE, 'TYPE) ALPHA_PREDICATE \<Rightarrow>
+   ('VALUE, 'TYPE) ALPHA_PREDICATE" where
+"p1 \<in> WF_ALPHA_PREDICATE \<and>
+ p2 \<in> WF_ALPHA_PREDICATE \<longrightarrow>
+ RefA p1 p2 = [p2 \<Rightarrow>\<alpha> p1]\<alpha>"
+
+notation RefA (infix "\<sqsubseteq>\<alpha>" 100)
+
+subsection {* Meta-logical Operators *}
+
+definition TautologyA ::
+  "('VALUE, 'TYPE) ALPHA_PREDICATE \<Rightarrow> bool" where
+"p \<in> WF_ALPHA_PREDICATE \<longrightarrow>
+ TautologyA p \<longleftrightarrow> (p = true (\<alpha> p))"
+
+notation TautologyA ("taut _" [50] 50)
+
+definition ContradictionA ::
+  "('VALUE, 'TYPE) ALPHA_PREDICATE \<Rightarrow> bool" where
+"p \<in> WF_ALPHA_PREDICATE \<longrightarrow>
+ ContradictionA p \<longleftrightarrow> (p = false (\<alpha> p))"
+
+notation ContradictionA ("contra _" [50] 50)
+
+definition RefinementA ::
+  "('VALUE, 'TYPE) ALPHA_PREDICATE \<Rightarrow>
+   ('VALUE, 'TYPE) ALPHA_PREDICATE \<Rightarrow> bool" where
+"p1 \<in> WF_ALPHA_PREDICATE \<and>
+ p2 \<in> WF_ALPHA_PREDICATE \<and>
+ (\<alpha> p1) = (\<alpha> p2) \<longrightarrow>
+ RefinementA p1 p2 \<longleftrightarrow> taut (p1 \<sqsubseteq>\<alpha> p2)"
+
+notation RefinementA (infix "\<sqsubseteq>" 50)
+
+subsection {* Theorems *}
+
+subsubsection {* Validation of Soundness *}
+
+theorem TrueA_noteq_FalseA :
+"a \<in> WF_ALPHABET \<Longrightarrow> true a \<noteq> false a"
+apply (simp add: TrueA_def FalseA_def)
+apply (simp add: TrueP_noteq_FalseP)
+done
+end
+end
