theories/generic/utp_types.thy
@@ -24,13 +24,23 @@ types ('VALUE, 'TYPE) BINDING =
 types ('VALUE, 'TYPE) BINDING_SET =
   "('VALUE, 'TYPE) BINDING set"
 
+types ('VALUE, 'TYPE) BINDING_BFUN =
+  "('VALUE, 'TYPE) BINDING \<Rightarrow> bool"
+
 types ('VALUE, 'TYPE) BINDING_FUN =
   "('VALUE, 'TYPE) BINDING \<Rightarrow> 'VALUE"
 
 types ('VALUE, 'TYPE) PREDICATE =
   "('VALUE, 'TYPE) BINDING_SET"
 
-types ('VALUE, 'TYPE) ALPHA_FUNCTION =
+types ('VALUE, 'TYPE) FUNCTION =
   "('VALUE, 'TYPE) PREDICATE \<Rightarrow>
    ('VALUE, 'TYPE) PREDICATE"
+
+types ('VALUE, 'TYPE) ALPHA_PREDICATE =
+  "('TYPE ALPHABET) \<times> ('VALUE, 'TYPE) PREDICATE"
+
+types ('VALUE, 'TYPE) ALPHA_FUNCTION =
+  "('VALUE, 'TYPE) ALPHA_PREDICATE \<Rightarrow>
+   ('VALUE, 'TYPE) ALPHA_PREDICATE"
 end
