theories/utp_meta.thy
@@ -15,7 +15,8 @@ imports utp_common
   "generic/utp_pred"
   "generic/utp_subst"
   "generic/utp_rel"
-  "generic/utp_laws"
+(*  "generic/utp_laws" *)
+  "alpha/utp_alpha_pred"
   "utils/utp_eval_pred"
   "utils/utp_eval_rel"
 begin
